fr.inria.atlanmod.coqtl.coq/core/Model.v
@@ -7,12 +7,12 @@ Scheme Equality for list.
 
 Class Model (Node: Type) (Edge: Type) :=
   {
-    modelElements : list Node;
+    modelNodes : list Node;
     modelLinks : list Edge;
   }.
 
 Definition allNodes {Node: Type} {Edge: Type} (m: Model Node Edge) : list Node :=
-  (@modelElements _ _ m).
+  (@modelNodes _ _ m).
 
 Definition allEdges {Node: Type} {Edge: Type} (m: Model Node Edge) : list Edge :=
   (@modelLinks _ _ m).
@@ -24,5 +24,5 @@ Definition allEdges {Node: Type} {Edge: Type} (m: Model Node Edge) : list Edge :
  *)
 
 Definition Model_beq {ME ML: Type} (ME_beq: ME -> ME -> bool) (ML_beq: ML -> ML -> bool) (m1 m2: Model ME ML) :=
-  andb (list_beq ME_beq (@modelElements _ _ m1) (@modelElements _ _ m2))
+  andb (list_beq ME_beq (@modelNodes _ _ m1) (@modelNodes _ _ m2))
   (list_beq ML_beq (@modelLinks _ _ m1) (@modelLinks _ _ m2)).
